Clean up for submission, prove associativity of lifted substitution

Term.thy
@@ -2,10 +2,7 @@ theory Term
   imports Unification
 begin
 
-
-term "Var ''a''"
-term "Fun (1::nat) [Var ''a'']"
-
+subsection \<open>Assignment 5\<close>
 
 datatype symbol = Const string | iota | Hash | Pair | Senc | Aenc | Sign
 
@@ -19,9 +16,6 @@ datatype msg = Const string
   | Sign msg msg ("[_]\<^sub>_" [57,57]56)
 
 value "\<lbrace>\<langle>a,\<h>(b)\<rangle>\<rbrace>\<^sub>c = Senc (Pair a \<h> b) c"
-
-
-term "msg.Hash a"
                      
 fun arity :: "symbol \<Rightarrow> nat" where
 "arity (symbol.Const _)= 0"
@@ -79,14 +73,26 @@ lemma type_definition_msg:
 
 setup_lifting type_definition_msg
 
+type_synonym equation_msg = "msg \<times> msg"
+type_synonym system_msg = "equation_msg list"
+
+
 lift_definition fv_msg::"msg \<Rightarrow> string set" is fv
   done
 
-lemma "fv_msg (msg.Variable ''a'') = {''a''}"
-  apply(simp add:fv_msg_def)
+lift_definition fv_eq_msg::"equation_msg \<Rightarrow> string set" is fv_eq
+  done
+
+lift_definition fv_sys_msg::"system_msg \<Rightarrow> string set" is fv_sys
   done
 
 type_synonym subst_msg = "string \<Rightarrow> msg"
+
+lift_definition sdom_msg::"subst_msg \<Rightarrow> string set" is sdom
+  done
+
+lift_definition svran_msg::"subst_msg \<Rightarrow> string set" is svran
+  done
 
 lift_definition sapply_msg::"subst_msg \<Rightarrow> msg \<Rightarrow> msg" is sapply
   by (simp add: wf_term_sapply)
@@ -104,23 +110,33 @@ lemma [simp]: "Variable \<circ>\<^sub>s \<tau> = \<tau>"
   by(auto simp add: scomp_msg_def map_fun_def comp_def var_term)
 
 lemma scomp_msg_assoc: "scomp_msg (\<sigma> \<circ>\<^sub>s \<tau>) \<rho> =  \<sigma> \<circ>\<^sub>s (\<tau> \<circ>\<^sub>s \<rho>)"
-  sorry
+  apply transfer
+  using scomp_assoc by blast
 
+fun embed_subst::"subst_msg \<Rightarrow> (symbol, string)subst" where
+"embed_subst \<sigma> m = embed (\<sigma> m)"
 
-type_synonym equation_msg = "msg \<times> msg"
-type_synonym system_msg = "equation_msg list"
+fun subst_to_subst_msg::"(symbol, string) subst \<Rightarrow> subst_msg" where
+"subst_to_subst_msg \<sigma> s =  msg_of_term (\<sigma> s)"
+
 
 fun embed_eqn::"equation_msg \<Rightarrow> (symbol, string) equation" where
 "embed_eqn (m1, m2) = (embed m1, embed m2)"
 
+fun msg_eqn_of_eqn::"(symbol, string) equation \<Rightarrow> equation_msg" where
+"msg_eqn_of_eqn (u,t) = (msg_of_term u, msg_of_term t)"
+
 fun embed_sys::"system_msg \<Rightarrow> (symbol,string) system" where
 "embed_sys sys = map embed_eqn sys"
+
+fun msg_sys_of_sys::"(symbol,string) system \<Rightarrow> system_msg" where
+"msg_sys_of_sys sys = map msg_eqn_of_eqn sys"
 
 lift_definition sapply_eq_msg::"subst_msg \<Rightarrow> equation_msg \<Rightarrow> equation_msg" is sapply_eq
   by (simp add: pred_prod_beta sapply_eq_def  wf_term_sapply)
 
-(*lift_definition sapply_sys_msg::"subst_msg \<Rightarrow> system_msg \<Rightarrow> system_msg" is sapply_sys
-  *)   
+definition sapply_sys_msg::"subst_msg \<Rightarrow> system_msg \<Rightarrow> system_msg" where
+"sapply_sys_msg \<sigma> sys = msg_sys_of_sys (sapply_sys (embed_subst \<sigma>) (embed_sys sys))"
 
 lift_definition unifies_msg::"subst_msg \<Rightarrow> equation_msg \<Rightarrow> bool" is unifies
   done
@@ -128,18 +144,7 @@ lift_definition unifies_msg::"subst_msg \<Rightarrow> equation_msg \<Rightarrow>
 lift_definition unifiess_msg::"subst_msg \<Rightarrow> system_msg \<Rightarrow> bool" is unifiess 
   done
 
-(*Why abstraction violation for subst_to_subst_msg when generating code for unify_msg?*)
-fun subst_to_subst_msg::"(symbol, string) subst \<Rightarrow> subst_msg" where
-"subst_to_subst_msg \<sigma> s =  msg_of_term (\<sigma> s)"
 
-
-(*lemma "wf_subst arity \<sigma> \<Longrightarrow> unifies_msg (subst_to_subst_msg \<sigma>) eqn \<longleftrightarrow> unifies \<sigma> (embed_eqn eqn)"
-  unfolding unifies_msg_def map_fun_def map_prod_def comp_def 
-  apply(simp)
-  apply auto
-   apply (metis case_prod_unfold embed_eqn.simps surjective_pairing)
-  by (metis case_prod_Pair_iden case_prod_map_prod embed_eqn.elims map_prod_simp)
-*)
 
 fun unify_msg::"system_msg \<Rightarrow> subst_msg option" where
 "unify_msg sys = (case (unify (embed_sys sys)) of Some \<sigma> \<Rightarrow> Some (subst_to_subst_msg \<sigma>) | None \<Rightarrow> None)"
@@ -151,11 +156,15 @@ proof -
   from assms
   obtain \<tau> where "unify (embed_sys sys) = Some \<tau>" by fastforce
   hence "unifiess \<tau> (embed_sys sys)" using unify_correct by blast
-  from assms have "\<sigma> = subst_to_subst_msg \<tau>" using \<open>unify (embed_sys sys) = Some \<tau>\<close> by auto
-  thm unifies_msg_def
-  with assms show ?thesis unfolding unifiess_msg_def map_fun_def comp_def map_prod_def 
-    using \<open>unifiess \<tau> (embed_sys sys)\<close>
+  moreover from assms have "\<sigma> = subst_to_subst_msg \<tau>" using \<open>unify (embed_sys sys) = Some \<tau>\<close> by auto
+  with assms show ?thesis
     sorry
 qed
+
+
+lemma lemma3_msg:
+  assumes "unify_msg sys = Some \<sigma>"
+  shows 1: "fv_sys_msg (sapply_sys_msg \<sigma> sys) \<subseteq> fv_sys_msg sys \<and> sdom_msg \<sigma> \<subseteq> fv_sys_msg sys \<and> svran_msg \<sigma> \<subseteq> fv_sys_msg sys"
+  sorry
 
 end
